Wavelet/Determinacy/Determinism.lean
@@ -26,7 +26,7 @@ theorem proc_indexed_guarded_step_unique_label
     case step.step.idx_guard.idx_guard =>
     cases hguard₁ <;> cases hguard₂
       <;> simp [Label.IsYieldOrSilentAndDet] at hdet
-    case spec_yield_ghost.spec_yield_ghost =>
+    case spec_yield.spec_yield =>
       have := Config.IndexedStep.unique_index hstep₁ hstep₂
         (by
           constructor; simp
@@ -36,12 +36,13 @@ theorem proc_indexed_guarded_step_unique_label
           have ⟨h₁, h₂, h₃⟩ := hyield₁
           have ⟨h₁', h₂', h₃'⟩ := hyield₂
           simp [← h₁] at h₁'
-          subst h₁'
+          have ⟨h₁₁', h₁₂'⟩ := h₁'
+          subst h₁₁' h₁₂'
           have := HEq.trans h₂ h₂'.symm
-          simp [Vector.push_eq_push] at this
-          replace this := Vector.inj_map (by simp [Function.Injective]) this.2
-          subst this
-          rename_i outputVals₁' _ outputVals₂'
+          simp at this
+          have ⟨h₁, h₂⟩ := this
+          subst h₁
+          rename_i outputVals₁' _ outputVals₂' _ _ _
           have : outputVals₁' = outputVals₂' := by
             symm
             apply hdet
@@ -50,43 +51,15 @@ theorem proc_indexed_guarded_step_unique_label
           rw [← heq_eq_eq _ _]
           apply HEq.trans h₃.symm h₃')
       simp at this
-      have ⟨⟨h₁, h₂, h₃⟩, _⟩ := this
-      subst h₁
-      simp [Vector.push_eq_push] at h₂
-      replace h₂ := Vector.inj_map (by simp [Function.Injective]) h₂.2
-      subst h₂
-      simp [Vector.push_eq_push] at h₃
-      replace h₃ := Vector.inj_map (by simp [Function.Injective]) h₃.2
+      have ⟨⟨⟨h₁, h₂⟩, h₃, h₄⟩, _⟩ := this
+      subst h₁ h₂
+      simp at h₃
+      have ⟨h₃₁, h₃₂⟩ := h₃
+      subst h₃₁
+      simp [Vector.push_eq_push] at h₄
+      replace h₃ := Vector.inj_map (by simp [Function.Injective]) h₄.2
       subst h₃
       rfl
-    case spec_yield.spec_yield =>
-      have := Config.IndexedStep.unique_index hstep₁ hstep₂
-        (by
-          and_intros
-          · simp
-          · simp
-          · intros op inputs outputs₁ outputs₂ hyield₁ hyield₂
-            simp at hyield₁ hyield₂
-            have ⟨h₁, h₂, h₃⟩ := hyield₁
-            have ⟨h₁', h₂', h₃'⟩ := hyield₂
-            subst h₁ h₂ h₃
-            simp at h₁'
-            subst h₁'
-            simp at h₂' h₃'
-            subst h₃'
-            have := Vector.inj_map (by simp [Function.Injective]) h₂'
-            subst this
-            congr
-            apply hdet
-            rfl
-            rfl)
-      simp at this
-      have ⟨⟨h₁, h₂, h₃⟩, _⟩ := this
-      subst h₁
-      simp at h₂ h₃
-      replace h₂ := Vector.inj_map (by simp [Function.Injective]) h₂
-      replace h₃ := Vector.inj_map (by simp [Function.Injective]) h₃
-      simp [h₂, h₃]
     any_goals rfl
     any_goals
       have := Config.IndexedStep.unique_index hstep₁ hstep₂
@@ -178,25 +151,16 @@ theorem proc_indexed_unguarded_step_det_label_mod
   rename_i l₁' l₂'
   cases l₁ <;> cases l₂ <;> simp at hl₁ hl₂
   case yield.yield =>
-    cases hguard₁ <;> cases hguard₂
-    case triv_yield_ghost.triv_yield_ghost =>
-      simp [Label.EqModYieldOutputs] at heq ⊢
-      have ⟨h₁, h₂⟩ := heq
-      subst h₁
-      simp [Vector.push_eq_push] at h₂
-      replace h₂ := Vector.inj_map (by simp [Function.Injective]) h₂.2
-      subst h₂
-      simp
+    cases hguard₁
+    cases hguard₂
     case triv_yield.triv_yield =>
       simp [Label.EqModYieldOutputs] at heq ⊢
-      have ⟨h₁, h₂⟩ := heq
-      subst h₁; simp at h₂
-      replace h₂ := Vector.inj_map (by simp [Function.Injective]) h₂
-      subst h₂
+      have ⟨⟨h₁, h₂⟩, h₃⟩ := heq
+      subst h₁ h₂
+      simp at h₃
+      replace h₃ := h₃.1
+      subst h₃
       simp
-    case triv_yield_ghost.triv_yield |
-      triv_yield.triv_yield_ghost =>
-      simp [Label.EqModYieldOutputs] at heq
   any_goals cases hguard₁ <;> cases hguard₂
   any_goals simp [Label.EqModYieldOutputs] at heq ⊢
 
@@ -219,7 +183,7 @@ theorem proc_indexed_unguarded_step_det_mod
   · constructor
     · cases hstep₂ <;> simp
     · cases hguard₁ <;> cases hguard₂
-      case triv_yield_ghost.triv_yield_ghost =>
+      case triv_yield.triv_yield =>
         intros op inputVals outputVals₁ outputVals₂ hyield₁ hyield₂
         simp at hyield₁ hyield₂
         have ⟨h₁, h₂, h₃⟩ := hyield₁
@@ -230,21 +194,6 @@ theorem proc_indexed_unguarded_step_det_mod
         apply Vector.forall₂_to_forall₂_push_toList
         · simp [EqModGhost]
         · simp [EqModGhost]
-      case triv_yield.triv_yield =>
-        intros op inputVals outputVals₁ outputVals₂ hyield₁ hyield₂
-        simp at hyield₁ hyield₂
-        have ⟨h₁, h₂, h₃⟩ := hyield₁
-        have ⟨h₁', h₂', h₃'⟩ := hyield₂
-        subst h₁
-        simp at h₂ h₃ h₂' h₃'
-        simp [← h₃, ← h₃', EqModGhost]
-      case triv_yield_ghost.triv_yield |
-        triv_yield.triv_yield_ghost =>
-        intros _ _ _ _ hyield₁ hyield₂
-        simp at hyield₁ hyield₂
-        have ⟨h₁, _⟩ := hyield₁
-        have ⟨h₁', _⟩ := hyield₂
-        simp [← h₁] at h₁'
       case triv_join.triv_join =>
         intros op inputVals outputVals₁ outputVals₂ hyield₁ hyield₂
         simp at hyield₁ hyield₂
