Wavelet/Determinacy/DisjointTokens.lean
@@ -573,27 +573,24 @@ theorem Config.DisjointTokens.guarded_inv
         apply PCM.framePreserving.from_le
         simp [Vector.toList_map]
         exact async_op_interp_le_tok_sum hntok_aop hinterp
-    | spec_yield_ghost =>
+    | spec_yield =>
       -- Normal operators with ghost tokens
       cases hstep with | step_op hmem hpop =>
-      rename_i op inputVals outputVals chans' inputs outputs
+      rename_i op ghost inputVals outputVals hpre chans' inputs outputs
       have hdisj' := pop_vals_disj_toks hdisj hpop
       constructor
       · exact hntok
       · apply push_vals_disj_toks
         apply ChanMap.DisjointWith.imp_frame_preserving _ hdisj'
-        simp [Vector.toList_push, Vector.toList_map, asTok]
-        apply hfp
-    | spec_yield =>
-      -- Normal operators w/o ghost tokens
-      cases hstep with | step_op hmem hpop =>
-      rename_i op inputVals outputVals chans' inputs outputs
-      have hdisj' := pop_vals_disj_toks hdisj hpop
-      constructor
-      · exact hntok
-      · apply push_vals_disj_toks
-        apply ChanMap.DisjointWith.imp_frame_preserving _ hdisj'
-        simp [Vector.toList_map, PCM.framePreserving]
+        cases ghost with
+        | true =>
+          simp [Vector.toList_push, Vector.toList_map, asTok, WithSpec.opInputs]
+          apply hfp
+        | false =>
+          simp at hpre
+          simp [Vector.toList_push, Vector.toList_map, asTok, WithSpec.opInputs]
+          simp [← hpre]
+          apply hfp
     | spec_join houtputs₀ houtputs₁ hsum =>
       rename_i k l req rem inst toks vals outputVals
       -- Join
